Derived.v
@@ -1,0 +1,236 @@
+Require Import Coq.Lists.List.
+Require Import Coq.Program.Equality.
+
+Require Import KA.Terms.
+Require Import KA.Finite.
+Require Import KA.Main.
+Require Import KA.Scope.
+Local Open Scope ka_scope.
+
+Section DerivedBase.
+  Variable (A: Type).
+  Context `{Finite A}.
+  Notation term := (term A).
+
+  Lemma starstar (a: A):
+    ($ a) * * == ($ a)*
+  .
+  Proof.
+    apply completeness; auto; split; intros.
+    - apply term_matches_star_split in H0.
+      apply term_matches_star_split.
+      destruct H0 as [l [? ?]]; subst.
+      induction l.
+      + now exists nil.
+      + destruct IHl as [l' [? ?]].
+        * intros.
+          apply H1.
+          now right.
+        * specialize (H1 a0 ltac:(now left)).
+          apply term_matches_star_split in H1.
+          destruct H1 as [l'' [? ?]]; subst.
+          exists (l'' ++ l').
+          rewrite concat_app, <- H0.
+          intuition.
+          apply in_app_iff in H1.
+          destruct H1; intuition.
+    - replace w with (w ++ nil) by (now rewrite app_nil_r).
+      apply MatchStarStep; auto.
+      apply MatchStarBase.
+  Qed.
+
+  Lemma slide (a b: A):
+    ($ a ;; $ b)* ;; $a == $a ;; ($ b ;; $ a)*
+  .
+  Proof.
+    apply completeness; auto; split; intros.
+    - dependent destruction H0.
+      apply term_matches_star_repeat in H0_.
+      destruct H0_ as [n ?].
+      revert w1 w2 H0 H0_0; induction n;
+      autorewrite with term_repeat; intros.
+      + dependent destruction H0.
+        rewrite app_nil_l, <- app_nil_r.
+        apply MatchTimes; auto.
+        apply MatchStarBase.
+      + dependent destruction H0.
+        dependent destruction H0_.
+        repeat rewrite <- app_assoc.
+        apply MatchTimes; auto.
+        specialize (IHn _ _ H0_0 H0_3).
+        dependent destruction IHn.
+        rewrite <- x.
+        rewrite app_assoc.
+        * apply MatchStarStep; auto.
+          now apply MatchTimes.
+    - dependent destruction H0.
+      apply term_matches_star_repeat in H0_0.
+      destruct H0_0 as [n ?].
+      revert w1 w2 H0 H0_; induction n;
+      autorewrite with term_repeat; intros.
+      + dependent destruction H0.
+        rewrite app_nil_r,  <- app_nil_l.
+        apply MatchTimes; auto.
+        apply MatchStarBase.
+      + dependent destruction H0.
+        dependent destruction H0_.
+        specialize (IHn _ _ H0_0 H0_2).
+        dependent destruction IHn.
+        repeat rewrite <- app_assoc.
+        rewrite <- x.
+        repeat rewrite app_assoc.
+        apply MatchTimes; auto.
+        apply MatchStarStep; auto.
+        now apply MatchTimes.
+  Qed.
+
+  Lemma denest_pre (a b: A):
+    ($ a)* ;; ($b ;; ($ a)*)* <= ($ a + $ b)*
+  .
+  Proof.
+    apply EFixLeft.
+    apply term_lequiv_split.
+    - rewrite EStarLeft at 2.
+      rewrite EStarLeft at 3.
+      apply term_lequiv_split_left.
+      fold_term_lequiv.
+      apply times_mor_mono.
+      + unfold term_lequiv.
+        apply term_lequiv_split_left.
+        apply term_lequiv_refl.
+      + apply term_lequiv_refl.
+    - rewrite <- ETimesUnitRight with (t := ($ b ;; ($ a)*)*).
+      apply EFixLeft.
+      apply term_lequiv_split.
+      + rewrite EStarLeft with (t := $a + $b).
+        apply term_lequiv_split_left.
+        fold_term_lequiv.
+        rewrite <- ETimesAssoc.
+        apply times_mor_mono.
+        * unfold term_lequiv.
+          apply term_lequiv_split_right.
+          apply term_lequiv_refl.
+        * rewrite EDistributeLeft.
+          apply term_lequiv_split.
+          -- apply EFixLeft.
+             apply term_lequiv_split.
+             ++ rewrite EStarLeft with (t := $a + $b) at 2.
+                rewrite EStarLeft with (t := $a + $b) at 3.
+                apply term_lequiv_split_left.
+                fold_term_lequiv.
+                apply times_mor_mono.
+                ** apply term_lequiv_split_left.
+                   apply term_lequiv_refl.
+                ** apply term_lequiv_refl.
+             ++ rewrite EStarLeft with (t := $a + $b) at 2.
+                rewrite EStarLeft with (t := $a + $b) at 3.
+                apply term_lequiv_split_left.
+                apply term_lequiv_refl.
+          -- apply EFixLeft.
+             apply term_lequiv_split.
+             ++ rewrite EStarLeft with (t := $a + $b) at 2.
+                rewrite EStarLeft with (t := $a + $b) at 3.
+                apply term_lequiv_split_left.
+                fold_term_lequiv.
+                apply times_mor_mono.
+                ** apply term_lequiv_split_left.
+                   apply term_lequiv_refl.
+                ** apply term_lequiv_refl.
+             ++ rewrite EStarLeft with (t := $a + $b).
+                apply term_lequiv_split_right.
+                apply term_lequiv_refl.
+      + rewrite EStarLeft with (t := $a + $b).
+        apply term_lequiv_split_right.
+        apply term_lequiv_refl.
+  Qed.
+
+  Lemma denest (a b: A):
+    ($ a + $ b)* == ($ a)* ;; ($b ;; ($ a)*) *
+  .
+  Proof.
+    apply completeness; auto; split; intros.
+    - apply term_matches_star_repeat in H0.
+      destruct H0 as [n ?].
+      revert w H0; induction n;
+      autorewrite with term_repeat; intros.
+      + dependent destruction H0.
+        rewrite <- app_nil_l.
+        apply MatchTimes; apply MatchStarBase.
+      + dependent destruction H0.
+        dependent destruction H0_.
+        * apply IHn in H0_0.
+          dependent destruction H0_0.
+          rewrite app_assoc.
+          apply MatchTimes; auto.
+          apply MatchStarStep; auto.
+        * apply IHn in H0_0.
+          dependent destruction H0_0.
+          rewrite app_assoc.
+          rewrite <- app_nil_l.
+          apply MatchTimes; [apply MatchStarBase|].
+          apply MatchStarStep; auto.
+          apply MatchTimes; auto.
+    - eapply term_lequiv_sound.
+      + apply denest_pre.
+      + auto.
+  Qed.
+End DerivedBase.
+
+Section DerivedProper.
+  Variable (A: Type).
+  Variable (a1 a2: A).
+  Context `{Finite A}.
+  Hypotheses (HDiff: a1 <> a2).
+  Notation term := (term A).
+
+  Definition subst2 (t1 t2: term) (a: A) : term :=
+    if finite_dec a1 a then t1
+    else if finite_dec a2 a then t2
+    else 0
+  .
+
+  Ltac force_subst_check :=
+    autorewrite with term_subst; unfold subst2; simpl;
+    pose proof HDiff;
+    repeat destruct (finite_dec _ _); subst; try contradiction;
+    reflexivity.
+
+  Lemma denest_general (t1 t2: term):
+    (t1 + t2)* == t1* ;; (t2 ;; t1*) *
+  .
+  Proof.
+    replace ((t1 + t2)*)
+      with (term_subst (subst2 t1 t2) (($a1 + $a2)*))
+      by force_subst_check.
+    replace (t1 *;; (t2;; t1 *) *)
+      with (term_subst (subst2 t1 t2) ($a1 *;; ($a2;; $a1 *) *))
+      by force_subst_check.
+    now apply term_subst_preserve, denest.
+  Qed.
+
+  Lemma starstar_general (t: term):
+    t * * == t*
+  .
+  Proof.
+    replace (t * *)
+      with (term_subst (subst2 t t) ($a1 * *))
+      by force_subst_check.
+    replace (t*)
+      with (term_subst (subst2 t t) ($a1*))
+      by force_subst_check.
+    now eapply term_subst_preserve, starstar.
+  Qed.
+
+  Lemma slide_general (t1 t2: term):
+    (t1 ;; t2)* ;; t1 == t1 ;; (t2 ;; t1)*
+  .
+  Proof.
+    replace ((t1 ;; t2)* ;; t1)
+      with (term_subst (subst2 t1 t2) (($a1 ;; $a2)* ;; $a1))
+      by force_subst_check.
+    replace (t1 ;; (t2 ;; t1)*)
+      with (term_subst (subst2 t1 t2) ($a1 ;; ($a2 ;; $a1)*))
+      by force_subst_check.
+    now eapply term_subst_preserve, slide.
+  Qed.
+End DerivedProper.
