Main.v
@@ -1,0 +1,70 @@
+Require Import Coq.Lists.List.
+
+Require Import KA.Finite.
+Require Import KA.Terms.
+Require Import KA.Structure.
+Require Import KA.Scope.
+Local Open Scope ka_scope.
+
+Section Main.
+  Variable (A: Type).
+  Context `{Finite A}.
+
+  Notation term := (term A).
+
+  Definition term_interp_finite_equiv
+    (t1 t2: term)
+  :=
+    forall {X: Type} `{Finite X} (k: kleene_algebra X) (f: A -> X),
+      kleene_interp k f t1 = kleene_interp k f t2
+  .
+
+  Theorem finite_model_property
+    (t1 t2: term)
+  :
+    term_interp_finite_equiv t1 t2 ->
+    t1 == t2
+  .
+  Proof.
+    intros.
+    rewrite term_normal_form_left with (t2 := t2) at 1; symmetry.
+    rewrite term_normal_form_right with (t1 := t1) at 1; symmetry.
+    rewrite H0.
+    - reflexivity.
+    - typeclasses eauto.
+  Qed.
+
+  Definition term_language_equiv
+    (t1 t2: term)
+  :=
+    forall w, term_matches t1 w <-> term_matches t2 w
+  .
+
+  Theorem completeness
+    (t1 t2: term)
+  :
+    term_language_equiv t1 t2 <->
+    t1 == t2
+  .
+  Proof.
+    split; intros.
+    - intros.
+      rewrite term_normal_form_left with (t2 := t2) at 1; symmetry.
+      rewrite term_normal_form_right with (t1 := t1) at 1; symmetry.
+      erewrite filter_ext.
+      + reflexivity.
+      + intros m.
+        apply ZMicromega.eq_true_iff_eq.
+        split; intros.
+        * apply kleene_interp_witness_construct in H1.
+          destruct H1 as [w [? ?]]; subst.
+          apply kleene_interp_witness_apply.
+          intuition.
+        * apply kleene_interp_witness_construct in H1.
+          destruct H1 as [w [? ?]]; subst.
+          apply kleene_interp_witness_apply.
+          intuition.
+    - unfold term_language_equiv; intros.
+      now apply term_equiv_sound.
+  Qed.
+End Main.
